DY/Step/Benchmark.lean
@@ -30,52 +30,87 @@ instance:
 
 
 def test: Traceful Unit := do
-  let _msg0 ← receive_message 0
-  let _msg1 ← receive_message 1
-  let _msg2 ← receive_message 2
-  let _msg3 ← receive_message 3
-  let _msg4 ← receive_message 4
-  let _msg5 ← receive_message 5
-  let _msg6 ← receive_message 6
-  let _msg7 ← receive_message 7
-  let _msg8 ← receive_message 8
-  let _msg9 ← receive_message 9
-  let _msg10 ← receive_message 10
-  let _msg11 ← receive_message 11
-  let _msg12 ← receive_message 12
-  let _msg13 ← receive_message 13
-  let _msg14 ← receive_message 14
-  let _msg15 ← receive_message 15
-  let _msg16 ← receive_message 16
-  let _msg17 ← receive_message 17
-  let _msg18 ← receive_message 18
-  let _msg19 ← receive_message 19
-  let _msg20 ← receive_message 20
-  let _msg21 ← receive_message 21
-  let _msg22 ← receive_message 22
-  let _msg23 ← receive_message 23
-  let _msg24 ← receive_message 24
-  let _msg25 ← receive_message 25
-  let _msg26 ← receive_message 26
-  let _msg27 ← receive_message 27
-  let _msg28 ← receive_message 28
-  let _msg29 ← receive_message 29
-  let _msg30 ← receive_message 30
-  let _msg31 ← receive_message 31
-  let _msg32 ← receive_message 32
-  let _msg33 ← receive_message 33
-  let _msg34 ← receive_message 34
-  let _msg35 ← receive_message 35
-  let _msg36 ← receive_message 36
-  let _msg37 ← receive_message 37
-  let _msg38 ← receive_message 38
-  let _msg39 ← receive_message 39
+  let msg0 ← receive_message 0
+  let msg1 ← receive_message 1
+  let msg2 ← receive_message 2
+  let msg3 ← receive_message 3
+  let msg4 ← receive_message 4
+  let msg5 ← receive_message 5
+  let msg6 ← receive_message 6
+  let msg7 ← receive_message 7
+  let msg8 ← receive_message 8
+  let msg9 ← receive_message 9
+  let msg10 ← receive_message 10
+  let msg11 ← receive_message 11
+  let msg12 ← receive_message 12
+  let msg13 ← receive_message 13
+  let msg14 ← receive_message 14
+  let msg15 ← receive_message 15
+  let msg16 ← receive_message 16
+  let msg17 ← receive_message 17
+  let msg18 ← receive_message 18
+  let msg19 ← receive_message 19
+  let msg20 ← receive_message 20
+  let msg21 ← receive_message 21
+  let msg22 ← receive_message 22
+  let msg23 ← receive_message 23
+  let msg24 ← receive_message 24
+  let msg25 ← receive_message 25
+  let msg26 ← receive_message 26
+  let msg27 ← receive_message 27
+  let msg28 ← receive_message 28
+  let msg29 ← receive_message 29
+  let msg30 ← receive_message 30
+  let msg31 ← receive_message 31
+  let msg32 ← receive_message 32
+  let msg33 ← receive_message 33
+  let msg34 ← receive_message 34
+  let msg35 ← receive_message 35
+  let msg36 ← receive_message 36
+  let msg37 ← receive_message 37
+  let msg38 ← receive_message 38
+  let msg39 ← receive_message 39
 
-  send_message _msg0
-
-
-set_option maxHeartbeats 10000000
-
+  send_message msg0
+  send_message msg1
+  send_message msg2
+  send_message msg3
+  send_message msg4
+  send_message msg5
+  send_message msg6
+  send_message msg7
+  send_message msg8
+  send_message msg9
+  send_message msg10
+  send_message msg11
+  send_message msg12
+  send_message msg13
+  send_message msg14
+  send_message msg15
+  send_message msg16
+  send_message msg17
+  send_message msg18
+  send_message msg19
+  send_message msg20
+  send_message msg21
+  send_message msg22
+  send_message msg23
+  send_message msg24
+  send_message msg25
+  send_message msg26
+  send_message msg27
+  send_message msg28
+  send_message msg29
+  send_message msg30
+  send_message msg31
+  send_message msg32
+  send_message msg33
+  send_message msg34
+  send_message msg35
+  send_message msg36
+  send_message msg37
+  send_message msg38
+  send_message msg39
 
 theorem test.spec:
   HoareTriple
@@ -83,9 +118,52 @@ theorem test.spec:
     (fun _ => True)
     (fun _ _ => True)
 := by
-  -- set_option trace.profiler true in
+  -- On TWal's laptop:
+  -- - full tactic executes in ~8s
+  -- - steps at the end take ~0.1s
+  -- TODO: investigate kernel checking time which seems slow
+  set_option trace.profiler true in
   apply HoareTriple.mk
   unfold test
+  step
+  step
+  step
+  step
+  step
+  step
+  step
+  step
+  step
+  step
+  step
+  step
+  step
+  step
+  step
+  step
+  step
+  step
+  step
+  step
+  step
+  step
+  step
+  step
+  step
+  step
+  step
+  step
+  step
+  step
+  step
+  step
+  step
+  step
+  step
+  step
+  step
+  step
+  step
   step
   step
   step
