DY/Trace.lean
@@ -2,3 +2,4 @@ module
 
 public import DY.Trace.Basic
 public import DY.Trace.Manipulation
+public meta import DY.Trace.Grind
